compiler/repl/evaluate_skipScript.sml
@@ -199,7 +199,7 @@ Proof
   \\ gs [SF SFY_ss]
 QED
 
-Theorem v_rel_update:
+Theorem v_rel_update_lemma:
   (∀fr ft fe v w.
     v_rel fr ft fe v w ⇒
       ∀fr1 ft1 fe1.
@@ -237,9 +237,9 @@ Proof
   \\ gs [SF SFY_ss]
 QED
 
-Theorem env_rel_update = CONJUNCT2 v_rel_update;
+Theorem env_rel_update = CONJUNCT2 v_rel_update_lemma;
 
-Theorem v_rel_update = CONJUNCT1 v_rel_update;
+Theorem v_rel_update = CONJUNCT1 v_rel_update_lemma;
 
 Theorem ctor_rel_nsAppend:
   ctor_rel ft fe x1.c x2.c ∧
